src/Rupicola/Examples/Cells/Swap.v
@@ -2,10 +2,12 @@ Require Import Rupicola.Lib.Api.
 Require Import Rupicola.Examples.Cells.Cells.
 
 Section with_parameters.
-  Context {width: Z} {BW: Bitwidth width} {word: word.word width} {mem: map.map word Byte.byte}.
+  Context {width: Z} {BW: Bitwidth width}.
+  Local Notation word := (bits width).
+  Context {mem: map.map word Byte.byte}.
   Context {locals: map.map String.string word}.
   Context {ext_spec: bedrock2.Semantics.ExtSpec}.
-  Context {word_ok : word.ok word} {mem_ok : map.ok mem}.
+  Context {mem_ok : map.ok mem}.
   Context {locals_ok : map.ok locals}.
   Context {ext_spec_ok : Semantics.ext_spec.ok ext_spec}.
 
@@ -35,4 +37,4 @@ Section with_parameters.
 End with_parameters.
 
 From bedrock2 Require Import BasicC64Semantics NotationsCustomEntry.
-Compute swap_br2fn. (* (word := word) *)
+Compute swap_br2fn. (* *)
