src/Rupicola/Examples/L64X128.v
@@ -7,14 +7,14 @@ Require Import Rupicola.Lib.Arrays.
 Require Import Rupicola.Lib.WordNotations.
 From bedrock2 Require Import BasicC64Semantics.
 
-Coercion co_word_of_Z := word.of_Z (word := word).
+Coercion co_word_of_Z := Zmod.of_Z (2 ^ 64).
 #[export] Hint Unfold co_word_of_Z : compiler_side_conditions.
 
 Definition M : word :=
-  word.of_Z 0xd1342543de82ef95.
+  bits.of_Z _ 0xd1342543de82ef95.
 
 Definition rotl (x: word) (k: Z) :=
-  (x <<w word.of_Z k) |w (x >>w word.of_Z (64 - k)).
+  (x <<w bits.of_Z _ k) |w (x >>w bits.of_Z _ (64 - k)).
 
 Definition lxm_next (a s: word) (x: list word) :=
   let/n x0 := ListArray.get x 0 in
