src/Rupicola/Examples/Loops.v
@@ -5,34 +5,36 @@ Require Import Rupicola.Examples.Cells.Cells.
 Import LoopCompiler.
 
 Section Ex.
-  Context {width: Z} {BW: Bitwidth width} {word: word.word width} {mem: map.map word Byte.byte}.
+  Context {width: Z} {BW: Bitwidth width}.
+  Local Notation word := (bits width).
+  Context {mem: map.map word Byte.byte}.
   Context {locals: map.map String.string word}.
   Context {ext_spec: bedrock2.Semantics.ExtSpec}.
-  Context {word_ok : word.ok word} {mem_ok : map.ok mem}.
+  Context {mem_ok : map.ok mem}.
   Context {locals_ok : map.ok locals}.
   Context {ext_spec_ok : Semantics.ext_spec.ok ext_spec}.
 
   Program Definition vect_memcpy {n1 n2} (len: word)
           (a1: VectorArray.t word n1)
           (a2: VectorArray.t word n2)
-          (pr1: word.unsigned len < Z.of_nat n1)
-          (pr2: word.unsigned len < Z.of_nat n2) :=
+          (pr1: Zmod.unsigned len < Z.of_nat n1)
+          (pr2: Zmod.unsigned len < Z.of_nat n2) :=
     let/n a2 := ranged_for_u
-                 (word.of_Z 0) len
+                 Zmod.zero len
                  (fun a2 tok idx Hlt =>
                     let/n v := VectorArray.get a1 idx _ in
                     let/n a2 := VectorArray.put a2 idx _ v in
                     (tok, a2)) a2 in
     (a1, a2).
   Next Obligation.
-    pose proof word.unsigned_range idx.
-    pose proof word.unsigned_range len.
+    pose proof bits.unsigned_range idx width_nonneg.
+    pose proof bits.unsigned_range len width_nonneg.
     unfold cast, Convertible_word_nat.
     lia.
   Qed.
   Next Obligation.
-    pose proof word.unsigned_range idx.
-    pose proof word.unsigned_range len.
+    pose proof bits.unsigned_range idx width_nonneg.
+    pose proof bits.unsigned_range len width_nonneg.
     unfold cast, Convertible_word_nat.
     lia.
   Qed.
@@ -41,8 +43,8 @@ Section Ex.
     fnspec! "vect_memcpy" (len: word) (a1_ptr a2_ptr : word) /
           {n1} (a1: VectorArray.t word n1)
           {n2} (a2: VectorArray.t word n2)
-          (pr1: word.unsigned len < Z.of_nat n1)
-          (pr2: word.unsigned len < Z.of_nat n2)
+          (pr1: Zmod.unsigned len < Z.of_nat n1)
+          (pr2: Zmod.unsigned len < Z.of_nat n2)
           R,
     { requires tr mem :=
         (vectorarray_value AccessWord a1_ptr a1 ⋆
@@ -64,25 +66,23 @@ Section Ex.
   Program Definition vect_memcpy_s {n1 n2} (len: word)
           (a1: VectorArray.t word n1)
           (a2: VectorArray.t word n2)
-          (pr1: word.signed len < Z.of_nat n1)
-          (pr2: word.signed len < Z.of_nat n2) :=
+          (pr1: Zmod.signed len < Z.of_nat n1)
+          (pr2: Zmod.signed len < Z.of_nat n2) :=
     let/n a2 := ranged_for_s
-                 (word.of_Z 0) len
+                 Zmod.zero len
                  (fun a2 tok idx Hlt =>
                     let/n v := VectorArray.get a1 idx _ in
                     let/n a2 := VectorArray.put a2 idx _ v in
                     (tok, a2)) a2 in
     (a1, a2).
   Next Obligation.
-    pose proof word.half_modulus_pos (word:=word).
     unfold cast, Convertible_word_nat.
-    rewrite word.signed_of_Z, word.swrap_inrange in H by lia.
+    rewrite Zmod.signed_0 in H.
     rewrite word.signed_gz_eq_unsigned; lia.
   Qed.
   Next Obligation.
-    pose proof word.half_modulus_pos (word:=word).
     unfold cast, Convertible_word_nat.
-    rewrite word.signed_of_Z, word.swrap_inrange in H by lia.
+    rewrite Zmod.signed_0 in H.
     rewrite word.signed_gz_eq_unsigned; lia.
   Qed.
 
@@ -90,8 +90,8 @@ Section Ex.
     fnspec! "vect_memcpy_s" (len: word) (a1_ptr a2_ptr : word) /
           {n1} (a1: VectorArray.t word n1)
           {n2} (a2: VectorArray.t word n2)
-          (pr1: word.signed len < Z.of_nat n1)
-          (pr2: word.signed len < Z.of_nat n2)
+          (pr1: Zmod.signed len < Z.of_nat n1)
+          (pr2: Zmod.signed len < Z.of_nat n2)
           R,
     { requires tr mem :=
         (vectorarray_value AccessWord a1_ptr a1 ⋆
@@ -114,7 +114,7 @@ Section Ex.
              (a1: ListArray.t word)
              (a2: ListArray.t word) :=
     let/n a2 := ranged_for_u
-                 (word.of_Z 0) len
+                 Zmod.zero len
                  (fun a2 tok idx Hlt =>
                     let/n v := ListArray.get a1 idx in
                     let/n a2 := ListArray.put a2 idx v in
@@ -125,8 +125,8 @@ Section Ex.
     fnspec! "sizedlist_memcpy" (len: word) (a1_ptr a2_ptr : word) /
           {n1} (a1: ListArray.t word)
           {n2} (a2: ListArray.t word)
-          (pr1: word.unsigned len < Z.of_nat n1)
-          (pr2: word.unsigned len < Z.of_nat n2)
+          (pr1: Zmod.unsigned len < Z.of_nat n1)
+          (pr2: Zmod.unsigned len < Z.of_nat n2)
           R,
     { requires tr mem :=
         (sizedlistarray_value AccessWord n1 a1_ptr a1 ⋆
@@ -152,8 +152,8 @@ Section Ex.
   Instance spec_of_unsizedlist_memcpy : spec_of "unsizedlist_memcpy" :=
     fnspec! "unsizedlist_memcpy" (len: word) (a1_ptr a2_ptr : word) /
           (a1: ListArray.t word) (a2: ListArray.t word)
-          (pr1: word.unsigned len <= Z.of_nat (List.length a1))
-          (pr2: word.unsigned len <= Z.of_nat (List.length a2))
+          (pr1: Zmod.unsigned len <= Z.of_nat (List.length a1))
+          (pr2: Zmod.unsigned len <= Z.of_nat (List.length a2))
           R,
     { requires tr mem :=
         (listarray_value AccessWord a1_ptr a1 ⋆
@@ -192,19 +192,19 @@ Section Ex.
   End Unsz.
 
   Program Definition incr_gallina (c: cell) : cell :=
-    let/n tick := word.of_Z 0 in
+    let/n tick := Zmod.zero in
     let/n (tick, c) :=
        ranged_for_u
-         (word.of_Z 3) (word.of_Z 5)
+         (bits.of_Z width 3) (bits.of_Z width 5)
          (fun '\< tick, c \> tok idx bounded =>
             let/n v := get c in
-            let/n v := word.add v idx in
+            let/n v := Zmod.add v idx in
             let/n c := put v in
-            let/n tick := word.add tick (word.of_Z 1) in
+            let/n tick := Zmod.add tick Zmod.one in
             (tok, \< tick, c \>))
          \< tick, c \> in
     (let/n v := get c in
-     let/n v := word.add v tick in
+     let/n v := Zmod.add v tick in
      let/n c := put v in
      c).
 
@@ -242,9 +242,9 @@ Module RangedForTests.
                              let acc := idx :: acc in
                              (t, acc)) []).
 
-  Time Compute (ranged_for_u (word.of_Z 0) (word.of_Z 15)
+  Time Compute (ranged_for_u Zmod.zero (bits.of_Z _ 15)
                           (fun acc t idx _ =>
-                             if word.ltu (word.of_Z 11) idx then
+                             if Semantics.ltu (bits.of_Z _ 11) idx then
                                let t' := ExitToken.break t in
                                (t', acc)
                              else
@@ -253,6 +253,6 @@ Module RangedForTests.
 End RangedForTests.
 
 From bedrock2 Require Import BasicC64Semantics NotationsCustomEntry.
-Compute sizedlist_memcpy_br2fn (word := word).
-Compute unsizedlist_memcpy_br2fn (word := word).
-Compute vect_memcpy_s_br2fn (word := word).
+Compute sizedlist_memcpy_br2fn (width := 64).
+Compute unsizedlist_memcpy_br2fn (width := 64).
+Compute vect_memcpy_s_br2fn (width := 64).
