src/Rupicola/Examples/Net/IPChecksum/IPChecksum.v
@@ -4,7 +4,7 @@ From Rupicola.Examples Require Import IPChecksum.Impl.
 Instance spec_of_ip_checksum : spec_of "ip_checksum" :=
   fnspec! "ip_checksum" data_ptr wlen / (data : list byte) R ~> chk,
     { requires tr mem :=
-        wlen = word.of_Z (Z.of_nat (length data)) /\
+        wlen = bits.of_Z _ (Z.of_nat (length data)) /\
         Z.of_nat (Datatypes.length data) < 2 ^ 32 /\
         (listarray_value AccessByte data_ptr data * R)%sep mem;
       ensures tr' mem' :=
