src/Rupicola/Examples/Uppercase.v
@@ -68,7 +68,7 @@ Section Upstr.
   Instance spec_of_upstr : spec_of "upstr" :=
     fnspec! "upstr" s_ptr wlen / (s : list byte) R,
       { requires tr mem :=
-          wlen = word.of_Z (Z.of_nat (length s)) /\
+          wlen = bits.of_Z _ (Z.of_nat (length s)) /\
           Z.of_nat (length s) < 2 ^ 64 /\
           (sizedlistarray_value AccessByte (length s) s_ptr s * R)%sep mem;
         ensures tr' mem' :=
